commit

AP/AP/Defense/Corner.lean
@@ -10,62 +10,124 @@ deriving Inhabited, DecidableEq
 
 namespace Corner
 
+variable {c c₁ c₂ : Corner}
+
 @[simp]
 def edge (dir : Dir) (offset : PointZ) : Edge where
   dir := dir
   offset := offset.coord dir
 
-def edge₁ (cor : Corner) : Edge :=
-  edge cor.dir cor.offset
+def edge₁ (c : Corner) : Edge :=
+  edge c.dir c.offset
 
-def edge₂ (cor : Corner) : Edge :=
-  edge cor.dir.rotRight cor.offset
+def edge₂ (c : Corner) : Edge :=
+  edge c.dir.rotRight c.offset
 
-def points (cor : Corner) : Set PointZ :=
-  cor.edge₁.points ∪ cor.edge₂.points
+def points (c : Corner) : Set PointZ :=
+  c.edge₁.points ∪ c.edge₂.points
 
-def memPoints (cor : Corner) (p : PointZ) : Bool :=
+def memPoints (c : Corner) (p : PointZ) : Bool :=
   let ⟨x, y⟩ := p
-  let ⟨cx, cy⟩ := cor.offset
-  match cor.dir with
+  let ⟨cx, cy⟩ := c.offset
+  match c.dir with
   | .up => y ≤ cy ∨ cx ≤ x
   | .right => cx ≤ x ∨ cy ≤ y
   | .down => cy ≤ y ∨ x ≤ cx
   | .left => x ≤ cx ∨ y ≤ cy
 
-theorem mem_points_iff_memPoints {cor : Corner} {p} :
-p ∈ cor.points ↔ cor.memPoints p := by
+theorem mem_points_iff_memPoints {p} :
+p ∈ c.points ↔ c.memPoints p := by
   simp [points, edge₁, edge₂, memPoints, Edge.points]
-  cases cor.dir <;> simp [Edge.memPoints]
+  cases c.dir <;> simp [Edge.memPoints]
 
-instance {cor : Corner} {p} : Decidable # p ∈ cor.points :=
-  match h : cor.memPoints p with
+instance {p} : Decidable # p ∈ c.points :=
+  match h : c.memPoints p with
   | true => .isTrue # by simp [mem_points_iff_memPoints, h]
   | false => .isFalse # by simp [mem_points_iff_memPoints, h]
 
 @[simp]
-theorem memPoints_eq {cor : Corner} {p} : cor.memPoints p = decide (p ∈ cor.points) := by
+theorem memPoints_eq {p} : c.memPoints p = decide (p ∈ c.points) := by
   simp [mem_points_iff_memPoints]
 
--- theorem points_inj {c₁ c₂ : Corner} (h : c₁.points = c₂.points) : c₁ = c₂ := by
+-- theorem points_inj (h : c₁.points = c₂.points) : c₁ = c₂ := by
 --   sorry
 
 -- @[simp]
--- theorem points_eq_points_iff {e₁ e₂ : Corner} : e₁.points = e₂.points ↔ e₁ = e₂ :=
+-- theorem points_eq_points_iff : c₁.points = c₂.points ↔ c₁ = c₂ :=
 --   ⟨points_inj, λ h => by rw [h]⟩
 
-def dist (cor : Corner) (p : PointZ) : ℤ :=
-  min (cor.edge₁.dist p) (cor.edge₂.dist p)
+def dist (c : Corner) (p : PointZ) : ℤ :=
+  min (c.edge₁.dist p) (c.edge₂.dist p)
 
-def defenseCnd (cor : Corner) (s : State) : Prop :=
-  6 ≤ cor.dist s.aPos ∧ ∀ (p : PointZ), cor.dist p = 0 →
-  7 ≤ p.dist cor.offset → p ∈ s.taken
+def defenseCnd (c : Corner) (s : State) : Prop :=
+  6 ≤ c.dist s.aPos ∧ ∀ (p : PointZ), c.dist p = 0 →
+  7 ≤ p.dist c.offset → p ∈ s.taken
 
-def defenseFn (cor : Corner) (s : State) : Option PointZ :=
-  cor.edge₁.defense.f s <|> cor.edge₂.defense.f s
+def defenseFn (c : Corner) (s : State) : Option PointZ :=
+  c.edge₁.defense.f s <|> c.edge₂.defense.f s
 
-def defense (cor : Corner) : Defense :=
-  { cnd := cor.defenseCnd
-  , ps := cor.points
-  , f := cor.defenseFn
+def defense (c : Corner) : Defense :=
+  { cnd := c.defenseCnd
+  , ps := c.points
+  , f := c.defenseFn
   }
+
+section min
+
+variable {α : Type*} [ha₁ : LinearOrder α]
+
+theorem _root_.le_of_le_min_left {a b c : α} (h : a ≤ min b c) : a ≤ b := by
+  rw [le_inf_iff] at h; exact h.1
+
+theorem _root_.le_of_le_min_right {a b c : α} (h : a ≤ min b c) : a ≤ c := by
+  rw [le_inf_iff] at h; exact h.2
+
+end min
+
+theorem cnd_defense_edge₁ {s} (h : c.defenseCnd s) : c.edge₁.defense.cnd s :=
+  le_of_le_min_left h.1
+
+theorem cnd_defense_edge₂ {s} (h : c.defenseCnd s) : c.edge₂.defense.cnd s :=
+  le_of_le_min_right h.1
+
+@[simp] theorem ps_defense : c.defense.ps = c.points := rfl
+@[simp] theorem f_defense : c.defense.f = c.defenseFn := rfl
+
+-- #check 0 #exit
+
+theorem wf_defense : c.defense.WF := by
+  constructor
+  intro s hs h a Ha d Hd n
+  have h₁ := cnd_defense_edge₁ h
+  have h₂ := cnd_defense_edge₂ h
+  have He₁ : c.edge₁.defense.WF; infer_instance
+  have He₂ : c.edge₂.defense.WF; infer_instance
+  generalize he₁ : c.edge₁.defense = e₁ at h₁ He₁
+  generalize he₂ : c.edge₂.defense = e₂ at h₂ He₂
+  rw [Defense.wf_def] at He₁ He₂
+  specialize He₁ s h₁ a (e₂.st d) n
+  specialize He₂ s h₂ a (e₁.st d) n
+  
+  generalize hr : sys.simulate (Strat.f ⟨a, e₁.st # e₂.st d⟩) s n = r at He₁
+  
+  have h₃ : sys.simulate (Strat.f ⟨a, e₂.st # e₁.st d⟩) s n = r
+  · rw [←hr]
+    apply sys.simulate_congr
+    sorry
+  
+  rw [h₃] at He₂; clear h₃
+  
+  have h₄ : sys.simulate (Strat.f ⟨a, c.defense.st d⟩) s n = r
+  · rw [←hr]
+    apply sys.simulate_congr
+    sorry
+  
+  rw [h₄]
+  subst he₁ he₂
+  simp at He₁ He₂
+  simp [points, He₁, He₂]
+
+-- #check 0 #exit
+
+@[simp]
+instance : c.defense.WF := wf_defense
